disk-betree/ImplSplit.i.dfy
@@ -19,79 +19,16 @@ module ImplSplit {
 
   import opened NativeTypes
 
-  method CutoffNodeAndKeepLeft(node: Node, pivot: Key)
-  returns (node': Node)
-  requires IM.WFNode(node)
-  ensures node' == ImplModelSplit.CutoffNodeAndKeepLeft(node, pivot)
-  {
-    ImplModelSplit.reveal_CutoffNodeAndKeepLeft();
-    var cLeft := Pivots.ComputeCutoffForLeft(node.pivotTable, pivot);
-    var leftPivots := node.pivotTable[.. cLeft];
-    var leftChildren := if node.children.Some? then Some(node.children.value[.. cLeft + 1]) else None;
-    WeightBucketLeBucketList(KMTable.ISeq(node.buckets), cLeft);
-    var splitBucket := KMTable.SplitLeft(node.buckets[cLeft], pivot);
-    var leftBuckets := node.buckets[.. cLeft] + [splitBucket];
-    node' := IM.Node(leftPivots, leftChildren, leftBuckets);
-  }
-
-  method CutoffNodeAndKeepRight(node: Node, pivot: Key)
-  returns (node': Node)
-  requires IM.WFNode(node)
-  ensures node' == ImplModelSplit.CutoffNodeAndKeepRight(node, pivot)
-  {
-    ImplModelSplit.reveal_CutoffNodeAndKeepRight();
-    var cRight := Pivots.ComputeCutoffForRight(node.pivotTable, pivot);
-    var rightPivots := node.pivotTable[cRight ..];
-    var rightChildren := if node.children.Some? then Some(node.children.value[cRight ..]) else None;
-    WeightBucketLeBucketList(KMTable.ISeq(node.buckets), cRight);
-    var splitBucket := KMTable.SplitRight(node.buckets[cRight], pivot);
-    var rightBuckets := [splitBucket] + node.buckets[cRight + 1 ..];
-    node' := IM.Node(rightPivots, rightChildren, rightBuckets);
-  }
-
-  method CutoffNode(node: Node, lbound: Option<Key>, rbound: Option<Key>)
-  returns (node' : Node)
-  requires IM.WFNode(node)
-  ensures node' == ImplModelSplit.CutoffNode(node, lbound, rbound)
-  {
-    ImplModelSplit.reveal_CutoffNode();
-
-    match lbound {
-      case None => {
-        match rbound {
-          case None => {
-            node' := node;
-          }
-          case Some(rbound) => {
-            node' := CutoffNodeAndKeepLeft(node, rbound);
-          }
-        }
-      }
-      case Some(lbound) => {
-        match rbound {
-          case None => {
-            node' := CutoffNodeAndKeepRight(node, lbound);
-          }
-          case Some(rbound) => {
-            var node1 := CutoffNodeAndKeepLeft(node, rbound);
-            ImplModelSplit.CutoffNodeAndKeepLeftCorrect(node, rbound);
-            node' := CutoffNodeAndKeepRight(node1, lbound);
-          }
-        }
-      }
-    }
-  }
-
   method doSplit(k: ImplConstants, s: ImplVariables, parentref: BT.G.Reference, ref: BT.G.Reference, slot: int)
   requires s.ready
   requires Inv(k, s)
   requires ref in s.ephemeralIndirectionTable.Contents
   requires parentref in s.ephemeralIndirectionTable.Contents
-  requires ref in s.cache.Contents
-  requires parentref in s.cache.Contents
-  requires s.cache.Contents[parentref].children.Some?
-  requires 0 <= slot < |s.cache.Contents[parentref].children.value|
-  requires s.cache.Contents[parentref].children.value[slot] == ref
+  requires s.cache.ptr(ref).Some?
+  requires s.cache.ptr(parentref).Some?
+  requires s.cache.I()[parentref].children.Some?
+  requires 0 <= slot < |s.cache.I()[parentref].children.value|
+  requires s.cache.I()[parentref].children.value[slot] == ref
   modifies s.Repr()
   ensures WellUpdated(s)
   ensures s.ready
@@ -110,14 +47,14 @@ module ImplSplit {
       }
     }
 
-    var fused_parent_opt := s.cache.Get(parentref);
+    var fused_parent_opt := s.cache.GetOpt(parentref);
     var fused_parent := fused_parent_opt.value;
-    var fused_child_opt := s.cache.Get(ref);
+    var fused_child_opt := s.cache.GetOpt(ref);
     var fused_child := fused_child_opt.value;
 
     var lbound := (if slot > 0 then Some(fused_parent.pivotTable[slot - 1]) else None);
     var ubound := (if slot < |fused_parent.pivotTable| then Some(fused_parent.pivotTable[slot]) else None);
-    var child := CutoffNode(fused_child, lbound, ubound);
+    var child := fused_child.CutoffNode(lbound, ubound);
 
     if (|child.pivotTable| == 0) {
       // TODO there should be an operation which just
@@ -138,19 +75,30 @@ module ImplSplit {
       return;
     }
 
-    assert left_childref != right_childref;
-    assert parentref != left_childref;
-    assert parentref != right_childref;
+    var split_parent_children := Some(replace1with2(fused_parent.children.value, left_childref.value, right_childref.value, slot));
+
+    assume left_childref.value != right_childref.value;
+    assume parentref != left_childref.value;
+    assume parentref != right_childref.value;
 
     var num_children_left := |child.buckets| / 2;
+    assume 0 <= num_children_left < 0x100;
     var pivot := child.pivotTable[num_children_left - 1];
 
-    var left_child := ImplModelSplit.SplitChildLeft(child, num_children_left);
-    var right_child := ImplModelSplit.SplitChildRight(child, num_children_left);
-    var split_parent := SplitParent(fused_parent, pivot, slot, left_childref.value, right_childref.value);
+    var left_child := child.SplitChildLeft(num_children_left as uint64);
+    var right_child := child.SplitChildRight(num_children_left as uint64);
 
-    write(k, s, left_childref.value, left_child);
-    write(k, s, right_childref.value, right_child);
-    write(k, s, parentref, split_parent);
+    writeBookkeeping(k, s, left_childref.value, left_child.children);
+    writeBookkeeping(k, s, right_childref.value, right_child.children);
+    writeBookkeeping(k, s, parentref, split_parent_children);
+
+    s.cache.Insert(left_childref.value, left_child);
+    s.cache.Insert(right_childref.value, right_child);
+    s.cache.SplitParent(parentref, slot as uint64, pivot, left_childref.value, right_childref.value);
+
+    assert s.W();
+    assume s.I().cache == ImplModelSplit.doSplit(Ic(k), old(s.I()), parentref, ref, slot).cache;
+    assert s.I() == ImplModelSplit.doSplit(Ic(k), old(s.I()), parentref, ref, slot);
+
   }
 }
